Add divisions, exp modulo, gcd

code/experimental/argmax/Hacl.Argmax.Common.fst
@@ -3,6 +3,7 @@ module Hacl.Argmax.Common
 open FStar.Math.Lemmas
 open FStar.Math.Lib
 open FStar.Constructive
+open FStar.Classical
 open FStar.Mul
 open FStar.Calc
 
@@ -26,32 +27,103 @@ let one = 1
 
 (* Basic algebra *)
 
+val mod_twice: x:int -> n:pos -> Lemma
+  ((x % n) % n = x % n)
+let mod_twice _ _ = ()
+
 val field_el: #n:big -> a:int -> bool
 let field_el #n a = a >= 0 && a < n
 
 type fe n = x:int{field_el #n x}
 
-val to_fe: #n:big -> a:nat -> r:fe n
+val to_fe: #n:big -> a:int -> r:fe n
 let to_fe #n a = lemma_mod_lt a n; a % n
 
 type binop = #n:big -> fe n -> fe n -> fe n
 val ( +% ): binop
-val ( *% ): binop
 let ( +% ) #n n1 n2 = (n1 + n2) % n
+
+val neg: #n:big -> a:fe n -> r:fe n{a +% r = 0}
+let neg #n a = if a = 0 then 0 else n - a
+
+val ( -% ): binop
+let ( -% ) #n n1 n2 = n1 +% neg n2
+
+val ( *% ): binop
 let ( *% ) #n n1 n2 = (n1 * n2) % n
 
 val sqr: #n:big -> fe n -> fe n
 let sqr #n a = a *% a
+
+val minus_is_neg: #n:big -> a:nat -> Lemma
+  (ensures ((-a%n) % n = neg (to_fe #n a)))
+let minus_is_neg #n a = ()
+
+val minus_is_neg2: #n:big -> a:fe n -> Lemma
+  (ensures (((-a)%n) = neg a))
+let minus_is_neg2 #n a = ()
+
+val add_comm: #n:big -> a:fe n -> b:fe n -> Lemma
+  (a +% b = b +% a)
+let add_comm #n _ _ = ()
 
 val mul_one: #n:big -> a:fe n -> Lemma
   (ensures (a *% one = a /\ one *% a = a))
   [SMTPat (one *% a); SMTPat (a *% one)]
 let mul_one #n a = ()
 
+val mul_neg: #n:big -> a:fe n -> b:fe n -> Lemma
+  (a *% (neg b) = neg (a *% b))
+let mul_neg #n a b =
+  admit ();
+  if b = 0 || a = 0 then ()
+  else
+    calc (==) {
+      a *% neg b;                         == { }
+      (a * (n - b)) % n;                  == { distributivity_sub_right a n b }
+      ((a * n) + (-(a * b))) % n;         == { modulo_distributivity (a * n) (-(a*b)) n }
+      ((a * n) % n + (-(a * b)) % n) % n; == { multiple_modulo_lemma a n }
+      ((-a * b) % n) % n;                 == { mod_twice (-(a*b)) n }
+      (-(a * b)) % n;
+    };
+    if a*b = 0 then assert ((-(a * b)) % n = 0)
+    else if a*b < n then begin
+      let c: fe n = a*b in
+      minus_is_neg2 c;
+      assert ((-c)%n = neg c)
+    end else admit()
+
 val mul_comm: #n:big -> a:fe n -> b:fe n -> Lemma
   (ensures (a *% b = b *% a))
   [SMTPat (a *% b)]
 let mul_comm #n a b = ()
+
+val mul_add_distr_r: #n:big -> a:fe n -> b:fe n -> c:fe n -> Lemma
+  (a *% (b +% c) = a *% b +% a *% c)
+let mul_add_distr_r #n _ _ _ = admit()
+
+val mul_add_distr_l: #n:big -> a:fe n -> b:fe n -> c:fe n -> Lemma
+  ((a +% b) *% c = a *% c +% b *% c)
+let mul_add_distr_l #n a b c = mul_add_distr_r c a b
+
+val mul_sub_distr_r: #n:big -> a:fe n -> b:fe n -> c:fe n -> Lemma
+  (a *% (b -% c) = a *% b -% a *% c)
+let mul_sub_distr_r #n a b c =
+    calc (==) {
+      a *% (b -% c);
+    == { }
+      a *% (b +% (neg c));
+    == { mul_add_distr_r a b (neg c) }
+      (a *% b) +% (a *% neg c);
+    == { mul_neg a c }
+      (a *% b) -% (a *% c);
+    }
+
+val mul_sub_distr_l: #n:big -> a:fe n -> b:fe n -> c:fe n -> Lemma
+  ((a -% b) *% c = a *% c -% b *% c)
+let mul_sub_distr_l #n a b c =
+  mul_sub_distr_r c a b;
+  mul_comm (a -% b) c
 
 val modulo_mul_distributivity: a:int -> b:int -> n:pos ->
     Lemma ((a * b) % n = ((a % n) * (b % n)) % n)
@@ -59,9 +131,6 @@ let rec modulo_mul_distributivity a b n =
   lemma_mod_mul_distr_l a b n;
   lemma_mod_mul_distr_r (a % n) b n
 
-val mod_twice: x:int -> n:pos -> Lemma
-  ((x % n) % n = x % n)
-let mod_twice _ _ = ()
 
 val mul3_modulo_out_l: #n:big -> a:fe n -> b:fe n -> c:fe n -> Lemma
   ((a *% b) *% c = ((a * b) * c) % n)
@@ -122,6 +191,68 @@ let mul4_assoc #n a b c d =
     (a *% c) *% (b *% d);
   }
 
+// Naive exp
+val nexp: #n:big -> fe n -> e:nat -> Tot (fe n) (decreases e)
+let rec nexp #n g e = match e with
+  | 0 -> 1
+  | 1 -> g
+  | _ -> g *% nexp g (e-1)
+
+val nexp_eq_arg1: #n:big -> g1:fe n -> g2:fe n -> e:nat -> Lemma
+  (requires (g1 = g2))
+  (ensures (nexp g1 e = nexp g2 e))
+let nexp_eq_arg1 #n _ _ _ = ()
+
+val nexp_one1: #n:big -> g:fe n -> Lemma
+  (ensures (nexp g one = g))
+  [SMTPat (nexp g one)]
+let nexp_one1 #n _ = ()
+
+val nexp_one2: #n:big -> e:nat -> Lemma
+  (ensures (nexp #n one e = one))
+  [SMTPat (nexp #n one e)]
+let rec nexp_one2 #n e = match e with
+  | 0 -> ()
+  | _ ->  nexp_one2 #n (e-1)
+
+val nexp_mul1: #n:big -> g:fe n -> e1:nat -> e2:nat -> Lemma
+  (nexp g e1 *% nexp g e2 = nexp g (e1 + e2))
+let rec nexp_mul1 #n g e1 e2 = match e2 with
+  | 0 -> assert(nexp g e2 = one)
+  | 1 -> assert(nexp g e2 = g)
+  | _ -> nexp_mul1 g e1 (e2-1)
+
+val nexp_mul2: #n:big -> g1:fe n -> g2:fe n -> e:nat -> Lemma
+  (ensures (nexp (g1 *% g2) e = nexp g1 e *% nexp g2 e))
+  (decreases g2)
+let rec nexp_mul2 #n g1 g2 e = match g2 with
+  | 0 -> (assert (g1 *% 0 = 0); assert (nexp g1 e *% 0 = 0))
+  | 1 -> begin
+    assert(g2 = one);
+    assert (g1 *% g2 = g1);
+    nexp_eq_arg1 (g1 *% g2) g1 e;
+    assert(nexp (g1 *% g2) e = nexp g1 e)
+    end
+  | _ -> begin
+    nexp_mul2 g1 (g2 -% one) e;
+    calc (==) {
+      g1 *% (g2 -% one);
+    == { mul_sub_distr_r g1 g2 one }
+      (g1 *% g2) -% g1;
+    };
+    admit();
+//    calc (==) {
+//      nexp g1 e *% nexp (g2 -% one) e;
+//    == { }
+//
+//    };
+    admit()
+    end
+
+val nexp_exp: #n:big -> g:fe n -> e1:nat -> e2:nat -> Lemma
+  ((nexp #n (nexp #n g e1) e2) = (nexp #n g (e1 * e2)))
+let nexp_exp #n _ _ _ = admit()
+
 
 // Define fexp' for composite n and for unit g.
 val fexp: #n:big -> fe n -> e:nat -> Tot (fe n) (decreases e)
@@ -133,20 +264,21 @@ let rec fexp #n g e =
      then fexp (g *% g) (e / 2)
      else fexp (g *% g) ((e - 1) / 2) *% g
 
-val fexp_mul1: #n:big -> g:fe n -> e1:nat -> e2:nat -> Lemma
-  (fexp g e1 *% fexp g e2 = fexp g (e1 + e2))
-let rec fexp_mul1 #n g e1 e2 = match e2 with
+val fexp_eq_nexp: #n:big -> g:fe n -> e:nat -> Lemma
+  (ensures (nexp g e = fexp g e)) (decreases e)
+let rec fexp_eq_nexp #n g e = match e with
   | 0 -> ()
-//  | 1 -> ()
-  | _ -> admit()
-
-val fexp_mul2: #n:big -> g1:fe n -> g2:fe n -> e:nat -> Lemma
-  (fexp (g1 *% g2) e = fexp g1 e *% fexp g2 e)
-let fexp_mul2 #n _ _ _ = admit()
-
-val fexp_exp: #n:big -> g:fe n -> e1:nat -> e2:nat -> Lemma
-  (fexp #n (fexp #n g e1) e2 = fexp #n g (e1 * e2))
-let fexp_exp #n _ _ _ = admit()
+  | 1 -> ()
+  | _ ->
+    if e % 2 = 0
+    then begin
+      fexp_eq_nexp #n (g *% g) (e/2);
+      nexp_exp #n g 2 (e/2)
+    end
+    else begin
+      fexp_eq_nexp #n (g *% g) ((e-1)/2);
+      nexp_exp g 2 ((e-1)/2)
+    end
 
 val fexp_one1: #n:big -> g:fe n -> Lemma
   (ensures (fexp g one = g))
@@ -156,13 +288,35 @@ let fexp_one1 #n _ = ()
 val fexp_one2: #n:big -> e:nat -> Lemma
   (ensures (fexp #n one e = one))
   [SMTPat (fexp #n one e)]
-let rec fexp_one2 #n e = match e with
-  | 0 -> ()
-  | _ ->  fexp_one2 #n (if e % 2 = 0 then e / 2 else (e - 1) / 2)
+let rec fexp_one2 #n e = fexp_eq_nexp #n one e; nexp_one2 #n e
+
+val fexp_mul1: #n:big -> g:fe n -> e1:nat -> e2:nat -> Lemma
+  (fexp g e1 *% fexp g e2 = fexp g (e1 + e2))
+let fexp_mul1 #n g e1 e2 =
+  fexp_eq_nexp g e1;
+  fexp_eq_nexp g e2;
+  fexp_eq_nexp g (e1+e2);
+  nexp_mul1 g e1 e2
+
+val fexp_mul2: #n:big -> g1:fe n -> g2:fe n -> e:nat -> Lemma
+  (fexp (g1 *% g2) e = fexp g1 e *% fexp g2 e)
+let fexp_mul2 #n g1 g2 e =
+  fexp_eq_nexp (g1 *% g2) e;
+  fexp_eq_nexp g1 e;
+  fexp_eq_nexp g2 e;
+  nexp_mul2 g1 g2 e
+
+val fexp_exp: #n:big -> g:fe n -> e1:nat -> e2:nat -> Lemma
+  (fexp #n (fexp #n g e1) e2 = fexp #n g (e1 * e2))
+let fexp_exp #n g e1 e2 =
+  fexp_eq_nexp g e1;
+  fexp_eq_nexp (nexp g e1) e2;
+  fexp_eq_nexp g (e1 * e2);
+  nexp_exp g e1 e2
 
 (* GCD and LCM *)
 
-type divides (a:pos) (b:pos) = cexists (fun (c:pos) -> a * c == b)
+type divides (a:pos) (b:pos) = exists (c:pos). a * c = b
 
 type is_gcd (a:pos) (b:pos) (gcd:pos) =
     (forall (d:pos). divides d a /\ divides d b ==> divides d gcd)
@@ -181,10 +335,20 @@ let rec ex_eucl a b =
 val gcd: a:pos -> b:pos -> Tot (r:pos{is_gcd a b r}) (decreases b)
 let gcd a b = Mktuple3?._1 (ex_eucl a b)
 
-val ex_eucl_lemma1: a:pos -> b:pos -> g:int -> u:int -> v:int -> Lemma
+val ex_eucl_lemma1: a:pos -> b:pos -> g:pos -> u:int -> v:int -> Lemma
   (requires (a * u + b * v = g))
-  (ensures (exists k. gcd a b = k * g))
+  (ensures (exists k. g = k * gcd a b))
 let ex_eucl_lemma1 a b g u v = admit()
+
+val ex_eucl_lemma2: a:pos -> b:pos -> g:pos -> u:int -> v:int -> Lemma
+  (requires (a * u + b * v = g /\ divides g a /\ divides g b))
+  (ensures (gcd a b = g))
+let ex_eucl_lemma2 a b g u v = admit()
+
+val ex_eucl_lemma3: a:pos -> b:pos -> u:int -> v:int -> Lemma
+  (requires (a * u + b * v = 1))
+  (ensures (gcd a b = 1))
+let ex_eucl_lemma3 a b u v = ex_eucl_lemma2 a b 1 u v
 
 val lcm: pos -> pos -> pos
 let lcm a b = abs ((a / gcd a b) * b)
@@ -259,35 +423,95 @@ let isunit_prod #n a b =
   assert((a *% b) *% (finv a *% finv b) = one);
   finv_unique (a *% b) (finv a *% finv b)
 
+val inv_as_gcd1: #n:big -> a:fe n{a>0} -> Lemma
+  (requires (gcd a n = 1))
+  (ensures (isunit a))
+let inv_as_gcd1 #n a =
+  let (g,u,v) = ex_eucl a n in
+  assert (gcd a n = g);
+
+  assert (g = 1);
+  assert (u*a + v*n = 1);
+  assert (u*a - 1 = -v*n);
+  assert (u*a - 1 = (-v)*n);
+  assert (u*a = 1 + (-v)*n);
+  assert (((u*a)%n = (1 + (-v)*n)%n));
+  modulo_distributivity 1 ((-v)*n) n;
+  assert ((u*a)%n = (1%n + ((-v)*n)%n)%n);
+  multiple_modulo_lemma (-v) n;
+  assert((((-v)*n)%n) = 0);
+  assert ((u*a)%n = (1%n + 0)%n);
+  assert ((u*a)%n = (1%n)%n);
+  mod_twice 1 n;
+  assert ((u*a)%n = (1%n));
+  assert ((u*a)%n = 1);
+  modulo_mul_distributivity u a n;
+  assert (((u%n)*(a%n))%n = 1);
+  assert (((to_fe #n u)*(a%n))%n = 1);
+  modulo_lemma a n;
+  assert(a%n = a);
+  assert ((to_fe #n u *% a) = 1);
+  assert (isunit a)
+
+val inv_as_gcd2: #n:big -> a:fe n{a>0} -> Lemma
+  (requires (isunit a))
+  (ensures (gcd a n = 1))
+let inv_as_gcd2 #n a =
+  let u = finv a in
+
+  assert (isunit a);
+  assert ((u *% a) = 1);
+  assert ((u * a)%n = 1);
+  assert ((u * a)%n = 1);
+  mod_prop n (u*a) 1;
+  assert ((u * a) - 1 = ((u*a)/n)*n);
+  assert ((u * a) - ((u*a)/n)*n = 1);
+  assert ((u * a) + (-(u*a)/n)*n = 1);
+  ex_eucl_lemma3 a n u (-(u*a)/n);
+  assert (gcd a n = 1)
+
 val inv_as_gcd: #n:big -> a:fe n{a>0} -> Lemma
   (isunit a <==> gcd a n = 1)
 let inv_as_gcd #n a =
-  let (g,u,v) = ex_eucl a n in
-  assert (gcd a n = g);
-  assert (g = 1 ==> u*a + v*n = 1);
-  assert (g = 1 ==> u*a - 1 = -v*n);
-  assert (g = 1 ==> u*a - 1 = (-v)*n);
-  assert (g = 1 ==> (u *% a) = 1);
-  mod_ops_props #n
-  admit()
+  move_requires inv_as_gcd1 a;
+  move_requires inv_as_gcd2 a
 
-val isunit_in_bigger: n1:big -> n2:big{n2 = (n2 / n1) * n1} -> a:fe n1{isunit a} -> Lemma
-  (isunit (to_fe #n2 a))
-let isunit_in_bigger n1 n2 a =
-  let m = n2 / n1 in
-  assert (n2 = m * n1);
-  let b = finv a in
-  assert (forall (c:fe n1{c > 1}).
-          a *% b = c <==> (mod_ops_props a b c; a * b - c = ((a*b)/n1) * n1));
-  assert (forall (c:fe n1{c > 1}).
-          a *% b = c <==> (mod_ops_props a b c; m * ((a * b) - c) = m * ((a*b)/n1) * n1));
-  assert (forall (c:fe n1{c > 1}).
-          a *% b = c <==> (mod_ops_props a b c; m * ((a * b) - c) = ((a*b)/n1) * n2));
-  assert (forall (c:fe n1{c > 1}).
-          a *% b = c <==> (mod_ops_props a b c; m * (a * b) - m * c = ((a*b)/n1) * n2));
-  assert (forall (c:fe n1{c > 1}).
-          a *% b = c <==> (mod_ops_props a b c; m * (a * b) - m * c = ((a*b)/n1) * n2));
-  assert (forall (c:fe n1{c > 1}).
-          a *% b = c <==> (mod_ops_props a b c; m * (a * b) - m * c = ((a*b)/n1) * n2));
+val mult_order:
+     #n:big
+  -> g:fe n{isunit g}
+  -> r:pos{ fexp g r = one /\
+            (forall (x:pos{x<r}). fexp g x <> one) /\
+            (g <> 0 ==> r >= 1)
+            }
+let mult_order #n g = admit()
 
-  admit ()
+val g_pow_order_reduc: #n:comp -> g:fe n{isunit g /\ g > 0} -> x:pos -> Lemma
+  (ensures (fexp g x = fexp g (x % mult_order g)))
+  (decreases x)
+let rec g_pow_order_reduc #n g x =
+  let r = mult_order g in
+  if x < r
+  then modulo_lemma x r
+  else begin
+    lemma_div_mod x r;
+    assert(x = r * (x / r) + x % r);
+    fexp_mul1 g (r * (x/r)) (x%r);
+    fexp_exp g r (x/r);
+    assert(fexp g r = one);
+    fexp_one2 #n (x/r)
+  end
+
+val g_pow_isunit: #n:comp -> g:fe n{isunit g /\ g > 0}  -> x:pos -> Lemma
+  (isunit (fexp g x))
+let g_pow_isunit #n g x =
+  let r = mult_order g in
+  let x' = x % r in
+  modulo_range_lemma x r;
+  let inv_e = r - x' in
+  assert(inv_e >= 0 && inv_e <= r);
+  assert(fexp g r = one);
+  g_pow_order_reduc g x;
+  fexp_mul1 g x' inv_e;
+  assert(fexp g x' *% fexp g (r - x') = one);
+  assert(fexp g x *% fexp g (r - x') = one);
+  finv_unique (fexp g x) (fexp g (r - x'))
